src/GoHoare.v
@@ -336,3 +336,126 @@ Qed.
 
 Hint Resolve sep_star_ptsto_some_find. (* TODO hintdb *)
 
+Inductive Declaration :=
+| Decl (T : Type) {Wr: GoWrapper T}.
+
+Arguments Decl T {Wr}.
+
+Fixpoint nth_var {n} m : n_tuple n var -> var :=
+  match n with
+  | 0 => fun _ => 0
+  | S n' =>
+    match m with
+    | 0 => fun t => fst t
+    | S m' => fun t => nth_var m' (snd t)
+    end
+  end.
+
+Definition decls_pre (decls : list Declaration) {n} (vars : n_tuple n var) : nat -> pred.
+  induction decls; intro m.
+  - exact emp.
+  - destruct a.
+    exact ((nth_var m vars ~>? T * IHdecls (S m))%pred).
+Defined.
+
+Lemma decls_pre_shift : forall decls n vars var0 m,
+  @decls_pre decls (S n) (var0, vars) (S m) <=p=> @decls_pre decls n vars m.
+Proof.
+  induction decls.
+  - reflexivity.
+  - intros. destruct a. simpl.
+    rewrite IHdecls.
+    reflexivity.
+Qed.
+
+Definition decls_post (decls : list Declaration) {n} (vars : n_tuple n var) : nat -> pred.
+  induction decls; intro m.
+  - exact emp.
+  - destruct a.
+    exact ((exists x, nth_var m vars |-> Val wrap_type x) * IHdecls (S m))%pred.
+Defined.
+
+Lemma decls_post_shift : forall decls n vars var0 m,
+  @decls_post decls (S n) (var0, vars) (S m) <=p=> @decls_post decls n vars m.
+Proof.
+  induction decls.
+  - reflexivity.
+  - intros. destruct a. simpl.
+    Check pimpl_sep_star.
+    rewrite IHdecls.
+    reflexivity.
+Qed.
+
+
+Lemma decls_pre_impl_post :
+  forall n decls vars m,
+    @decls_pre decls n vars m =p=> decls_post decls vars m.
+Proof.
+  induction decls; intros.
+  - auto.
+  - destruct a.
+    simpl.
+    rewrite IHdecls.
+    reflexivity.
+Qed.
+
+Record WrappedType :=
+  {
+    WrType : Type;
+    Wrapper : GoWrapper WrType;
+  }.
+
+Definition with_wrapper T {Wr : GoWrapper T} := {| WrType := T |}.
+Arguments with_wrapper T {Wr}.
+
+Instance WrapWrappedType (wt : WrappedType) : GoWrapper wt.(WrType).
+destruct wt.
+assumption.
+Defined.
+
+Fixpoint arg_tuple (args : list WrappedType) : Type :=
+  match args with
+  | [] => unit
+  | arg :: args' => (arg.(WrType) * arg_tuple args')%type
+  end.
+
+Fixpoint argval_foralls (args : list WrappedType) :
+  forall (B : arg_tuple args -> Prop), Prop :=
+  match args return forall (B : arg_tuple args -> Prop), Prop with
+  | [] => fun B => B tt
+  | arg :: args' => fun B => forall argval : arg.(WrType), argval_foralls args' (fun argvals' => B (argval, argvals'))
+  end.
+
+Theorem argval_inst : forall (args : list WrappedType) (B : arg_tuple args -> Prop),
+    argval_foralls args B -> forall argvals : arg_tuple args, B argvals.
+Proof.
+  induction args; simpl; intros.
+  - destruct argvals. auto.
+  - destruct argvals.
+    specialize (IHargs (fun argvals' => B (w, argvals')) (H w)).
+    auto.
+Qed.
+
+Theorem argval_inst' : forall (args : list WrappedType) (B : arg_tuple args -> Prop),
+    (forall argvals : arg_tuple args, B argvals) -> argval_foralls args B.
+Proof.
+  induction args; simpl; auto.
+Qed.
+
+Fixpoint args_pre args : forall (argvars : n_tuple (List.length args) var) (argvals : arg_tuple args), pred :=
+  match args return forall (argvars : n_tuple (List.length args) var) (argvals : arg_tuple args), pred with
+  | [] => fun _ _ => emp
+  | arg :: args' => fun argvars argvals =>
+                     let '(argvar, argvars') := argvars in
+                     let '(argval, argvals') := argvals in
+                     (argvar ~> argval * args_pre args' argvars' argvals')%pred
+  end.
+
+Fixpoint args_post args : forall (argvars : n_tuple (List.length args) var) (argvals : arg_tuple args), pred :=
+  match args return forall (argvars : n_tuple (List.length args) var) (argvals : arg_tuple args), pred with
+  | [] => fun _ _ => emp
+  | arg :: args' => fun argvars argvals =>
+                     let '(argvar, argvars') := argvars in
+                     let '(argval, argvals') := argvals in
+                     (argvar |-> moved_value (wrap argval) * args_post args' argvars' argvals')%pred
+  end.
